\newcommand{\Release}{}
\newcommand{\Slide}{}
\newcommand{\PrintLecture}{1}
\newcommand{\PrintSolution}{0}
\input{header_class.tex}
\input{../../tex/hss_lualatex.tex}
\input{../../tex/hss_moodle.tex}
\input{../../tex/hss_beamer.tex}

\begin{document}

\maketitle

\section{小テスト（\MyClass）}

\begin{quiz}{\MyClass}

\QuizShortAnswer
{
  $(-2x^3y)^3\times(-2x^3y)$を計算せよ。\\
  　\\%whole space
  解答例：答えが$3x^6y^2$のとき，3,6,2と半角数字で解答欄に記入する。
}
{
  $=(-2)^3(x^3)^3y^3\times(-2)x^3y$\\
  $=-8x^9y^3\times(-2)x^3y$\\
  $=\{(-8)\times(-2)\}x^{9+3}y^{3+1}$
  $=16x^{12}y^4$
}
{30}
{16*12*4}
{}
{}
{}

\QuizMultipleChoices
{
  $ax^2+bx+c$を平方完成せよ。
}
{
  $=a(x^2+\frac{b}{a}x)+c$\\
  $=a\{x^2+\frac{b}{a}x+(\frac{b}{2a})^2-(\frac{b}{2a})^2\}+c$\\
  $=a(x+\frac{b}{2a})^2-\frac{b^2-4ac}{4a}$
}
{40}
{ $a(x+\frac{b}{2a})^2+\frac{b^2-4ac}{2a}$}
{ $a(x+\frac{b}{2a})^2-\frac{b^2-4ac}{2a}$}
{ $a(x+\frac{b}{2a})^2+\frac{b^2-4ac}{4a}$}
{*$a(x+\frac{b}{2a})^2-\frac{b^2-4ac}{4a}$}

\QuizMultipleChoices
{
  $ax^2+bx+c=0$を解け。
}
{
  二次方程式の解の公式より，\\
  \[x=\frac{-b\pm\sqrt{b^2-4ac}}{2a}\]
}
{30}
{*$x=\frac{-b\pm\sqrt{b^2-4ac}}{2a}$}
{ $x=\frac{-b\pm\sqrt{b^2+4ac}}{2a}$}
{ $x=\frac{-b\pm\sqrt{b^2-4ac}}{a}$}
{ $x=\frac{-b\pm\sqrt{b^2+4ac}}{a}$}

\end{quiz}

\end{document}
